add details about objs, delete some useless content

certiucos/spec/obj/service_obj_create_spec.v
@@ -1,3 +1,4 @@
+
 Require Import include_frm.
 Require Import NPeano.
 Require Import os_code_defs.
@@ -11,77 +12,42 @@ Require Import ifun_spec.
 
 Local Open Scope list_scope.
 
-Definition sobjcre_get_idx
+Definition sobjcre_get_idx_err
+  (vl: vallist) (O1: osabst) (rst: option val * option osabst) :=
+  match rst with
+  | (opv, O_opt) =>
+      exists objs,
+        opv =  Some (Vint32 (Int.mone)) /\ 
+        get O1 absobjsid = Some (absobjs objs) /\
+        (~(exists idx attr,  get objs idx = Some (objnull, attr) /\ 0 <= Int.unsigned idx < MAX_OBJ_NUM) 
+         /\ O_opt = Some O1)
+  end.
+            
+Definition sobjcre_get_idx_ok
   (vl: vallist) (O1: osabst) (rst: option val * option osabst) :=
   match rst with
   | (opv, O_opt) =>
       exists vidx objs,
       vl = (vidx :: nil) /\
       opv = None /\
-      get O1 absobjsid = Some (absobjs objs) /\
-      ((  ((~(exists idx attr,  get objs idx = Some (objnull, attr) /\ 0 <= Int.unsigned idx < MAX_OBJ_NUM) /\
-                                         vidx = Vint32 (Int.repr 255)) \/
-                (exists idx attr,  get objs idx = Some (objnull, attr) /\ 0 <= Int.unsigned idx < MAX_OBJ_NUM /\
-                                            vidx = Vint32 idx)) /\
-          O_opt = Some O1) \/
-       ( ((~(exists idx attr,  get objs idx = Some (objnull, attr) /\ 0 <= Int.unsigned idx < MAX_OBJ_NUM) /\
-                                          vidx <> Vint32 (Int.repr 255)) \/
-                    (exists idx attr,  get objs idx = Some (objnull, attr) /\ 0 <= Int.unsigned idx < MAX_OBJ_NUM /\
-                                                vidx <> Vint32 idx)) /\
-          O_opt = None))
+        get O1 absobjsid = Some (absobjs objs) /\
+        (exists idx attr,
+            get objs idx = Some (objnull, attr) /\ 0 <= Int.unsigned idx < MAX_OBJ_NUM
+            /\ (vidx = Vint32 idx /\ O_opt = Some (set O1 absobjsid (absobjs (set objs idx (objholder, attr))))
+                \/ vidx <> Vint32 idx /\ O_opt = None
+        ))
   end.
-
-Definition sobjcre_idxerr
-  (vl: vallist) (O1: osabst) (rst: option val * option osabst) :=
-  match rst with
-  | (opv, O_opt) =>
-      exists vidx objs,
-      vl = (vidx :: nil) /\
-      get O1 absobjsid = Some (absobjs objs) /\
-      ~(exists idx attr,  get objs idx = Some (objnull, attr) /\ 0 <= Int.unsigned idx < MAX_OBJ_NUM) /\
-      vidx = Vint32 (Int.repr 255) /\
-      opv = Some (Vint32 (Int.mone)) /\
-      O_opt = Some O1
-  end.
-
-Definition sobjcre_set_hold
-  (vl: vallist) (O1: osabst) (rst: option val * option osabst) :=
-  match rst with
-  | (opv, O_opt) =>
-      exists idx objs attr,
-      vl = (Vint32 idx :: nil) /\
-      Vint32 idx <> Vint32 (Int.repr 255) /\
-      get O1 absobjsid = Some (absobjs objs) /\
-      get objs idx = Some (objnull, attr) /\
-      0 <= Int.unsigned idx < MAX_OBJ_NUM /\
-      opv = None /\
-      O_opt = Some (set O1 absobjsid (absobjs (set objs idx (objholder, attr))))
-  end.
-
-Definition sobjcre_hold_kobj
-  (vl: vallist) (O1: osabst) (rst: option val * option osabst) :=
-  match rst with
-  | (opv, O_opt) =>
-      exists idx objs,
-      vl = (Vint32 idx :: nil) /\
-      Vint32 idx <> Vint32 (Int.repr 255) /\
-      0 <= Int.unsigned idx < MAX_OBJ_NUM /\
-      get O1 absobjsid = Some (absobjs objs) /\
-      opv = None /\
-      ( (exists attr, get objs idx = Some (objholder, attr) /\  O_opt = Some O1) \/
-         ~(exists attr, get objs idx = Some (objholder, attr)) /\ O_opt = None )
-  end.
-
+              
 Definition sobjcre_create_err
   (vl: vallist) (O1: osabst) (rst: option val * option osabst) :=
   match rst with
   | (opv, O_opt) =>
-      exists idx objs attr,
+      exists idx objs oid attr,
       vl = (Vint32 idx :: Vnull :: nil) /\
       Vint32 idx <> Vint32 (Int.repr 255) /\
       0 <= Int.unsigned idx < MAX_OBJ_NUM /\
       get O1 absobjsid = Some (absobjs objs) /\
-      get objs idx = Some (objholder, attr) /\
+      get objs idx = Some (oid, attr) /\
       opv = Some (Vint32 Int.mone) /\
       O_opt = Some (set O1 absobjsid (absobjs (set objs idx (objnull, attr))))
   end.
@@ -90,25 +56,25 @@ Definition sobjcre_create_succ
   (vl: vallist) (O1: osabst) (rst: option val * option osabst) :=
   match rst with
   | (opv, O_opt) =>
-      exists idx objs attr ptr satt,
+      exists idx objs oid attr ptr satt,
       vl = (Vint32 idx :: Vptr ptr :: Vint32 satt :: nil) /\
       Vint32 idx <> Vint32 (Int.repr 255) /\
       0 <= Int.unsigned idx < MAX_OBJ_NUM /\
       get O1 absobjsid = Some (absobjs objs) /\
-      get objs idx = Some (objholder, attr) /\
+      get objs idx = Some (oid, attr) /\
       opv = Some (Vint32 idx) /\
       O_opt = Some (set O1 absobjsid (absobjs (set objs idx (objid ptr, satt))))
   end.
 
+(* the abstract program for the function **service_obj_create**  *) 
 Definition sobjcre (vl: vallist) :=
   match vl with
     vkatt :: vsatt :: vr_idx :: vr_cre :: nil =>
-    sobjcre_get_idx (| vr_idx :: nil |) ;;
-        (sobjcre_idxerr (| vr_idx :: nil |) ??
-              (sobjcre_set_hold (| vr_idx :: nil |) ;; kobjcre ( vkatt :: vr_cre :: nil) ;;
-                    sobjcre_hold_kobj (| vr_idx :: nil |) ;;
-                      (sobjcre_create_err (| vr_idx :: vr_cre :: nil |) ??
-                        sobjcre_create_succ (| vr_idx :: vr_cre :: vsatt :: nil |) ) ) )
+      sobjcre_get_idx_err (| nil |) ??
+        ((sobjcre_get_idx_ok (| vr_idx :: nil |) ;;
+          kobjcre (vkatt :: vr_cre :: nil) ;;
+          (sobjcre_create_err (| vr_idx :: vr_cre :: nil |) ??
+             sobjcre_create_succ (| vr_idx :: vr_cre :: vsatt :: nil |))))
   | _ => spec_abort
   end.
 
@@ -144,4 +110,3 @@ Definition new_osq_spec_list_ext :=
      ++ new_osq_spec_list).
 
 Definition OS_spec_ext :=  convert_spec new_osq_spec_list_ext.
-
