certiucos/proofs/obj/kernel_obj_oper_proof.v
@@ -51,6 +51,7 @@ Proof.
    absimp_abt_solver.
 Qed.
 
+(* the proof that the function **kernel_obj_oper** satisfies its specification *) 
 Lemma kernel_obj_oper_proof:
   forall vl p r logicl ct, 
     Some p =
