certiucos/proofs/obj/service_obj_create_proof.v
@@ -39,101 +39,128 @@ Require Import objaux_pure.
 Require Import seplog_pattern_tacs.
 Require Import hoare_assign_tac_ext.
 
-Lemma sobjcre_absimp_get_idx:
-  forall sch P vr_idx objs s0,
-   ((~(exists idx attr,  get objs idx = Some (objnull, attr) /\ 0 <= Int.unsigned idx < MAX_OBJ_NUM) /\
-                                         vr_idx = Vint32 (Int.repr 255)) \/
-                (exists idx attr,  get objs idx = Some (objnull, attr) /\ 0 <= Int.unsigned idx < MAX_OBJ_NUM /\
-                                            vr_idx = Vint32 idx )) ->
+Lemma sobjcre_absimp_get_idx_err:
+  forall sch P objs s0,
+    (~(exists idx attr,  get objs idx = Some (objnull, attr) /\ 0 <= Int.unsigned idx < MAX_OBJ_NUM)) ->
     can_change_aop P ->
     absinfer sch
-      (<|| sobjcre_get_idx (|vr_idx :: nil|);; s0 ||>  ** HObjs objs ** P)
-      (<|| s0 ||> ** HObjs objs ** P).
+      (<|| sobjcre_get_idx_err (| nil |) ?? s0 ||>  ** HObjs objs ** P)
+      (<|| END (Some (Vint32 (Int.mone))) ||> ** HObjs objs ** P).
 Proof.
   infer_solver 0%nat.
 Qed.
 
-Lemma sobjcre_absimp_get_idx_abt:
-  forall sch P vkatt vsatt vr_idx vr_cre objs,
-   ((~(exists idx attr,  get objs idx = Some (objnull, attr) /\ 0 <= Int.unsigned idx < MAX_OBJ_NUM) /\
-                                         vr_idx <> Vint32 (Int.repr 255)) \/
-                (exists idx attr,  get objs idx = Some (objnull, attr) /\ 0 <= Int.unsigned idx < MAX_OBJ_NUM /\
-                                            vr_idx <> Vint32 idx)) ->
+Lemma sobjcre_absimp_get_idx_ok:
+  forall sch P vkatt vsatt vr_idx vr_cre objs attr idx,
+    get objs idx = Some (objnull, attr) ->
+    0 <= Int.unsigned idx < MAX_OBJ_NUM ->
+    vr_idx = Vint32 idx ->
     can_change_aop P ->
     absinfer sch
       (<|| sobjcre ( vkatt :: vsatt :: vr_idx :: vr_cre :: nil) ||>  ** HObjs objs ** P)
-      (<|| ABORT ||> ** HObjs objs ** P).
+      (<|| kobjcre (vkatt :: vr_cre :: nil) ;;
+       (sobjcre_create_err (| vr_idx :: vr_cre :: nil|)
+          ?? sobjcre_create_succ (| vr_idx :: vr_cre :: vsatt :: nil|)) ||>
+         ** HObjs (set objs idx (objholder, attr)) ** P).
 Proof.
   intros.
   assert (Hc: can_change_aop (HObjs objs ** P)).
   can_change_aop_solver.
   eapply absinfer_trans; try eapply absinfer_seq_abt; eauto.
-  eapply absinfer_seq; eauto.
-  eapply absinfer_abt; eauto.
-  absimp_abt_solver.
-Qed.
-
-Lemma sobjcre_absimp_idxerr:
-  forall sch P vr_idx objs s0,
-    ~(exists idx attr,  get objs idx = Some (objnull, attr) /\ 0 <= Int.unsigned idx < MAX_OBJ_NUM) -> 
-    vr_idx = Vint32 (Int.repr 255) ->
-    can_change_aop P ->
-    absinfer sch
-      (<|| sobjcre_idxerr (| vr_idx :: nil |) ?? s0 ||>  ** HObjs objs ** P) 
-      (<|| END (Some (Vint32 Int.mone)) ||> ** HObjs objs ** P).
-Proof.
+  unfold sobjcre. 
+  eapply absinfer_choice2.
+  can_change_aop_solver.
+  clear -Hc. eauto.
+  intros; eauto. 
   infer_solver 0%nat.
 Qed.
 
-Lemma sobjcre_absimp_set_hold:
-  forall sch idx P objs attr s0 s1,
+Lemma sobjcre_absimp_get_idx_abt: 
+  forall sch P vr_idx objs attr idx s0,
     get objs idx = Some (objnull, attr) ->
-    Vint32 idx <> Vint32 (Int.repr 255) ->
     0 <= Int.unsigned idx < MAX_OBJ_NUM ->
+    vr_idx <> Vint32 idx ->
     can_change_aop P ->
     absinfer sch
-      (<|| s1 ?? (sobjcre_set_hold (| Vint32 idx :: nil |) ;; s0) ||>  ** HObjs objs ** P) 
-      (<|| s0 ||> ** HObjs (set objs idx (objholder, attr)) ** P).
-Proof.
-  infer_solver 1%nat.
-Qed.
-
-Lemma sobjcre_absimp_hold_kobj:
-  forall sch P idx attr objs s0,
-   get objs idx = Some (objholder, attr) ->
-   Vint32 idx <> Vint32 (Int.repr 255) ->
-   0 <= Int.unsigned idx < MAX_OBJ_NUM ->
-    can_change_aop P ->
-    absinfer sch
-      (<|| sobjcre_hold_kobj (| Vint32 idx :: nil |) ;; s0  ||>  ** HObjs objs ** P)
-      (<|| s0 ||> ** HObjs objs ** P).
-Proof.
-  infer_solver 0%nat.
-Qed.
-
-Lemma sobjcre_absimp_hold_kobj_abt:
-  forall sch P idx objs s0,
-   ~(exists attr, get objs idx = Some (objholder, attr)) ->
-   Vint32 idx <> Vint32 (Int.repr 255) ->
-   0 <= Int.unsigned idx < MAX_OBJ_NUM ->
-    can_change_aop P ->
-    absinfer sch
-      (<|| sobjcre_hold_kobj (| Vint32 idx :: nil |) ;; s0  ||>  ** HObjs objs ** P)
+      (<|| sobjcre_get_idx_err (|nil|)
+         ?? (sobjcre_get_idx_ok (| vr_idx :: nil|);; s0) ||>  ** HObjs objs ** P)
       (<|| ABORT ||> ** HObjs objs ** P).
 Proof.
    intros.
    simpljoin.
   assert (Hc: can_change_aop (HObjs objs ** P)).
   can_change_aop_solver.
+  eapply absinfer_trans; try (eapply absinfer_choice2).
+  can_change_aop_solver.
+  clear -Hc. eauto.
+  intros; eauto.
   eapply absinfer_trans; try eapply absinfer_seq_abt; eauto.
-  eapply absinfer_seq; eauto.
+  eapply absinfer_seq; can_change_aop_solver. 
   eapply absinfer_abt; eauto.
   absimp_abt_solver.
-Qed.
+Qed.   
+
+(* Lemma sobjcre_absimp_idxerr: *)
+(*   forall sch P vr_idx objs s0, *)
+(*     ~(exists idx attr,  get objs idx = Some (objnull, attr) /\ 0 <= Int.unsigned idx < MAX_OBJ_NUM) ->  *)
+(*     vr_idx = Vint32 (Int.repr 255) -> *)
+(*     can_change_aop P -> *)
+(*     absinfer sch *)
+(*       (<|| sobjcre_idxerr (| vr_idx :: nil |) ?? s0 ||>  ** HObjs objs ** P)  *)
+(*       (<|| END (Some (Vint32 Int.mone)) ||> ** HObjs objs ** P). *)
+(* Proof. *)
+(*   infer_solver 0%nat. *)
+(* Qed. *)
+
+(* Lemma sobjcre_absimp_set_hold: *)
+(*   forall sch idx P objs attr s0 s1, *)
+(*     get objs idx = Some (objnull, attr) -> *)
+(*     Vint32 idx <> Vint32 (Int.repr 255) -> *)
+(*     0 <= Int.unsigned idx < MAX_OBJ_NUM -> *)
+(*     can_change_aop P -> *)
+(*     absinfer sch *)
+(*       (<|| s1 ?? (sobjcre_set_hold (| Vint32 idx :: nil |) ;; s0) ||>  ** HObjs objs ** P)  *)
+(*       (<|| s0 ||> ** HObjs (set objs idx (objholder, attr)) ** P). *)
+(* Proof. *)
+(*   infer_solver 1%nat. *)
+(* Qed. *)
+
+(* Lemma sobjcre_absimp_hold_kobj: *)
+(*   forall sch P idx attr objs s0, *)
+(*    get objs idx = Some (objholder, attr) -> *)
+(*    Vint32 idx <> Vint32 (Int.repr 255) -> *)
+(*    0 <= Int.unsigned idx < MAX_OBJ_NUM -> *)
+(*     can_change_aop P -> *)
+(*     absinfer sch *)
+(*       (<|| sobjcre_hold_kobj (| Vint32 idx :: nil |) ;; s0  ||>  ** HObjs objs ** P) *)
+(*       (<|| s0 ||> ** HObjs objs ** P). *)
+(* Proof. *)
+(*   infer_solver 0%nat. *)
+(* Qed. *)
+
+(* Lemma sobjcre_absimp_hold_kobj_abt: *)
+(*   forall sch P idx objs s0, *)
+(*    ~(exists attr, get objs idx = Some (objholder, attr)) -> *)
+(*    Vint32 idx <> Vint32 (Int.repr 255) -> *)
+(*    0 <= Int.unsigned idx < MAX_OBJ_NUM -> *)
+(*     can_change_aop P -> *)
+(*     absinfer sch *)
+(*       (<|| sobjcre_hold_kobj (| Vint32 idx :: nil |) ;; s0  ||>  ** HObjs objs ** P) *)
+(*       (<|| ABORT ||> ** HObjs objs ** P). *)
+(* Proof. *)
+(*    intros. *)
+(*    simpljoin. *)
+(*   assert (Hc: can_change_aop (HObjs objs ** P)). *)
+(*   can_change_aop_solver. *)
+(*   eapply absinfer_trans; try eapply absinfer_seq_abt; eauto. *)
+(*   eapply absinfer_seq; eauto. *)
+(*   eapply absinfer_abt; eauto. *)
+(*   absimp_abt_solver. *)
+(* Qed. *)
 
 Lemma sobjcre_absimp_create_err:
-  forall sch idx P objs attr s0,
-    get objs idx = Some (objholder, attr) ->
+  forall sch idx P objs oid attr s0,
+    get objs idx = Some (oid, attr) ->
     Vint32 idx <> Vint32 (Int.repr 255) ->
     0 <= Int.unsigned idx < MAX_OBJ_NUM ->
     can_change_aop P ->
@@ -145,8 +172,8 @@ Proof.
 Qed.
 
 Lemma sobjcre_absimp_create_succ:
-  forall sch idx P ptr objs attr sattr s0,
-    get objs idx = Some (objholder, attr) ->
+  forall sch idx P ptr objs oid attr sattr s0,
+    get objs idx = Some (oid, attr) ->
     Vint32 idx <> Vint32 (Int.repr 255) ->
     0 <= Int.unsigned idx < MAX_OBJ_NUM ->
     can_change_aop P ->
@@ -157,6 +184,7 @@ Proof.
   infer_solver 1%nat.
 Qed.
 
+(* the proof that the function **service_obj_create** satisfies its specification *) 
 Lemma service_obj_create_Proof: 
   forall tid vl p r, 
     Some p =
@@ -174,7 +202,7 @@ Proof.
   rename v0 into vr_cre.
   rename i into vkatt.
   rename i0 into vsatt.
-
+  
   hoare forward prim.
   unfold AOBJ.
   unfold AObjs.
@@ -242,30 +270,14 @@ Proof.
     lets Hget_full: obj_get_not_null H H1 Hlen.
     rewrite Hlen in Hget_full.
     change (Z.of_nat ∘ MAX_OBJ_NUM) with MAX_OBJ_NUM in *.
-   hoare_lifts_trms_pre (Aop, absobjs).
-   assert (Hv: vr_idx =  V$ 255 \/ vr_idx <>  V$ 255) by tauto.
-    destruct Hv as [Hv | Hv].
-    2:{ 
-        eapply abscsq_rule.
-       apply noabs_oslinv.
-       eapply sobjcre_absimp_get_idx_abt; eauto.
-      can_change_aop_solver.
-      eapply absinfer_eq.
-      apply absabort_rule.
-      }
-(*     hoare_lifts_trms_pre (Aop, absobjs). *)
-    subst.
+    hoare_lifts_trms_pre (Aop, absobjs).
+    (*  hoare_lifts_trms_pre (Aop, absobjs). *)
     eapply abscsq_rule.
     apply noabs_oslinv.
-    eapply sobjcre_absimp_get_idx; eauto.
+    eapply sobjcre_absimp_get_idx_err; eauto.
     can_change_aop_solver.
     eapply absinfer_eq.
     instantiate (1:= Afalse).
-     eapply abscsq_rule.
-    apply noabs_oslinv.
-    eapply sobjcre_absimp_idxerr; eauto.
-    can_change_aop_solver.
-    eapply absinfer_eq.
     hoare forward prim.
     unfold AOBJ.
     unfold AObjs.
@@ -281,11 +293,12 @@ Proof.
     hoare_split_pure_all.
     destruct H9; tryfalse.
   }
+  
   (* nth_ObjArr_free_P *)
-    hoare unfold.
-    inverts H10.
-    rename v'28 into idx.
-    hoare_assert_pure (0 <= idx < MAX_OBJ_NUM).
+  hoare unfold.
+  inverts H10. (* eq. logicval*)
+  rename v'28 into idx.
+  hoare_assert_pure (0 <= idx < MAX_OBJ_NUM).
   {
     get_hsat Hsat. 
     sep_lifts_trms_in Hsat AObjArr.
@@ -327,20 +340,21 @@ Proof.
   clear H9.
   assert (Hif_false': Vint32 ($ idx) <> Vint32 ($ 255)).
   { lets Hif_false': semacc_int_eq_false Hif_false.
-     pure_auto.
-   }
+    pure_auto.
+  }
   assert (Hrgn: Int.ltu ($ idx) Int.zero = false /\ Int.ltu ($ idx) ($ MAX_OBJ_NUM) = true).
   { clear - Hy_range.
-     unfold MAX_OBJ_NUM in *.
-     int auto.
-   }
+    unfold MAX_OBJ_NUM in *.
+    int auto.
+  }
   destruct Hrgn as (Hrgn1 & Hrgn2).
+  
   (* efield (obj_arr ′ [os_code_defs.idx ′]) ptr =ₑ 〈 OS_EVENT ∗ 〉 service_obj_create.PlaceHolder;ₛ *)
   rename v'27 into objvll.
- hoare_assert_pure (length objvll = (∘ (MAX_OBJ_NUM))).
+  hoare_assert_pure (length objvll = (∘ (MAX_OBJ_NUM))).
   { get_hsat Hsat.
     sep_lifts_trms_in Hsat AObjArr.
-     eapply aobjarr_len_frm; eauto.  }
+    eapply aobjarr_len_frm; eauto.  }
   eapply pure_split_rule'; introv Hlen.
   hoare_lifts_trms_pre (Aop, AObjArr).
   eapply backward_rule1.
@@ -350,7 +364,7 @@ Proof.
   eauto.
   rewrite Hlen.
   eapply obj_rgn_idx_lt; eauto.
-
+  
   destruct Hy_range as (Hrgn_lt0 & Hrgn_lt1).
   hoare normal pre.
   hoare_ex_intro.
@@ -362,9 +376,9 @@ Proof.
   apply Int.unsigned_range_2.
 
   rewrite Int.unsigned_repr in *;
-  try solve [clear -Hrgn_lt0 Hrgn_lt1; unfold MAX_OBJ_NUM in *; int auto].
+    try solve [clear -Hrgn_lt0 Hrgn_lt1; unfold MAX_OBJ_NUM in *; int auto].
   assert (Hget_null:
-            exists att, get objs ($ idx) = Some (objnull, att) /\ V_ObjPtr objvl = Some Vnull).
+           exists att, get objs ($ idx) = Some (objnull, att) /\ V_ObjPtr objvl = Some Vnull).
   {
     eapply obj_getnull; eauto.
   }
@@ -372,42 +386,11 @@ Proof.
   assert (Hidx_eq: Int.unsigned ($ idx) = idx).
   {
     rewrite Int.unsigned_repr in *;
-    try solve [clear -Hrgn_lt0 Hrgn_lt1; unfold MAX_OBJ_NUM in *; int auto].
-   }
-
-
-     hoare_lifts_trms_pre (Aop, absobjs).
-    assert (Hv: vr_idx = Vint32 ($ idx) \/ vr_idx <> Vint32 ($ idx)) by tauto.
-    destruct Hv as [Hv | Hv].
-    (* vr_idx <> Vint32 ($ idx) *)
-    2: {
-      eapply abscsq_rule.
-      apply noabs_oslinv.
-      eapply sobjcre_absimp_get_idx_abt; eauto.
-      right. do 2 eexists. splits; eauto.
-      rewrite Hidx_eq; auto.
-      can_change_aop_solver.
-      eapply absinfer_eq.
-      apply absabort_rule.
-    }
-    subst.
-    eapply abscsq_rule.
-    apply noabs_oslinv.
-    eapply sobjcre_absimp_get_idx; eauto.
-    right. do 2 eexists. splits; eauto.
-    rewrite Hidx_eq; auto.
-    can_change_aop_solver.
-    eapply absinfer_eq.
-
-    eapply abscsq_rule.
-    apply noabs_oslinv.
-    eapply sobjcre_absimp_set_hold; eauto.
-    rewrite Hidx_eq; auto.
-    can_change_aop_solver.
-    eapply absinfer_eq.
-
-   lets Hsplit : H9.
-   eapply new_array_type_vallist_match_split in Hsplit; eauto.
+      try solve [clear -Hrgn_lt0 Hrgn_lt1; unfold MAX_OBJ_NUM in *; int auto].
+  }
+  
+  lets Hsplit : H9.
+  eapply new_array_type_vallist_match_split in Hsplit; eauto.
   destruct Hsplit as (Hsp1 & Hsp2 & Hsp).
   lets Hvl: struct_type_vallist_match_elim_2 Hsp.
   destruct Hvl as (vatt & vp & Heq). subst.
@@ -415,35 +398,59 @@ Proof.
   inverts Hvatt.
   rewrite Hget_null in Hget; inverts Hget.
 
-    (* actual assign *)
+  (* actual assign *)
   unfold service_obj_create.PlaceHolder.
   hoare forward.
   hoare_assign_array_struct.
   { unfold AOSTCBPrioTbl.
-     introv Hsat.
-     eapply cast_rv_tptr.
-     eapply addrof_gvar_rv.
-     apply astar_l_anotinlenv_intro.
-     sep cancel (Agvarenv' OSPlaceHolder).
-     eauto.
-     {
-     sep_lifts_trms_in Hsat A_dom_lenv.
-     apply astar_l_adomlenv_elim in Hsat.
-     destruct Hsat as (Hlenv & _).
-     clear -Hlenv.
-     unfolds in Hlenv.
-     unfold EnvMod.indom.
-     pure_auto.
-     destruct H as ((l & t) & H).
-     assert (Hf: ~ListSet.set_In (OSPlaceHolder, t)
-                           ((satt, long)
-           :: (katt, Int16u) :: (idx, long) :: (y, char_t) :: (p, OS_EVENT ∗) :: nil)).
-     simpl; pure_auto; tryfalse.
-     rewrite Hlenv in Hf.
-     pure_auto.
+    introv Hsat.
+    eapply cast_rv_tptr.
+    eapply addrof_gvar_rv.
+    apply astar_l_anotinlenv_intro.
+    sep cancel (Agvarenv' OSPlaceHolder).
+    eauto.
+    {
+      sep_lifts_trms_in Hsat A_dom_lenv.
+      apply astar_l_adomlenv_elim in Hsat.
+      destruct Hsat as (Hlenv & _).
+      clear -Hlenv.
+      unfolds in Hlenv.
+      unfold EnvMod.indom.
+      pure_auto.
+      destruct H as ((l & t) & H).
+      assert (Hf: ~ListSet.set_In (OSPlaceHolder, t)
+                    ((satt, long)
+                       :: (katt, Int16u) :: (idx, long) :: (y, char_t) :: (p, OS_EVENT ∗) :: nil)).
+      simpl; pure_auto; tryfalse.
+      rewrite Hlenv in Hf.
+      pure_auto.
     }
     simpl; auto.
-   }
+  }
+
+  hoare_lifts_trms_pre (Aop, absobjs).
+  assert (Hv: vr_idx = Vint32 ($ idx) \/ vr_idx <> Vint32 ($ idx)) by tauto.
+  destruct Hv as [Hv | Hv].
+  (* vr_idx <> Vint32 ($ idx) *)
+  2: {
+    eapply abscsq_rule.
+    apply noabs_oslinv.
+    fold sobjcre.
+    eapply sobjcre_absimp_get_idx_abt; eauto.
+    splits; eauto; 
+    rewrite Hidx_eq; auto. 
+    can_change_aop_solver.
+    eapply absinfer_eq.
+    apply absabort_rule.
+  }
+  subst.
+  eapply abscsq_rule.
+  apply noabs_oslinv.
+  eapply sobjcre_absimp_get_idx_ok; eauto.
+  splits; eauto; rewrite Hidx_eq; auto.
+  can_change_aop_solver.
+  eapply absinfer_eq.
+  
   eapply backward_rule1.
   introv Hsat.
   eapply AObjArr_select_sn_ex_strong.
@@ -476,6 +483,7 @@ Proof.
   eapply OBJ_AUX_P_null_holder_preserve; eauto.
   eapply RH_OBJ_ECB_P_set_to_hold; eauto.
   pure_auto.
+  
   (* p ′ =ᶠ kernel_obj_create (·katt ′·);ₛ *)
   change (Vint32 vkatt :: vr_cre :: nil) with ((Vint32 vkatt :: nil) ++ (vr_cre :: nil)).
   hoare forward.
@@ -511,32 +519,12 @@ Proof.
   unfold AObjs.
   hoare unfold.
   rename v'51 into objs'.
-  hoare_lifts_trms_pre (Aop, absobjs).
-  assert (Hhold: (exists attr, get objs' ($ idx) = Some (objholder, attr)) \/
-                          ~(exists attr, get objs' ($ idx) = Some (objholder, attr) )) by tauto.
-  destruct Hhold as [Hhold | Habt].
-   2: {
-      eapply abscsq_rule.
-      apply noabs_oslinv.
-      eapply sobjcre_absimp_hold_kobj_abt; eauto.
-      rewrite Hidx_eq; auto.
-      can_change_aop_solver.
-      eapply absinfer_eq.
-      apply absabort_rule.
-    }
-   destruct Hhold as (attr & Hget').
-    eapply abscsq_rule.
-    apply noabs_oslinv.
-    eapply sobjcre_absimp_hold_kobj; eauto.
-    rewrite Hidx_eq; auto.
-    can_change_aop_solver.
-    eapply absinfer_eq.
-
+  
   rename v'50 into objvll.
- hoare_assert_pure (length objvll = (∘ (MAX_OBJ_NUM))).
+  hoare_assert_pure (length objvll = (∘ (MAX_OBJ_NUM))).
   { get_hsat Hsat.
     sep_lifts_trms_in Hsat AObjArr.
-     eapply aobjarr_len_frm; eauto.  }
+    eapply aobjarr_len_frm; eauto.  }
   eapply pure_split_rule'; introv Hlen'.
   hoare_lifts_trms_pre (Aop, AObjArr).
   eapply backward_rule1.
@@ -557,19 +545,17 @@ Proof.
   apply Int.unsigned_range_2.
 
   lets Hsplit : H18.
-   eapply new_array_type_vallist_match_split in Hsplit; eauto.
+  eapply new_array_type_vallist_match_split in Hsplit; eauto.
   destruct Hsplit as (Hsp1' & Hsp2' & Hsp').
   lets Hvl: struct_type_vallist_match_elim_2 Hsp'.
   destruct Hvl as (vatt & vp & Heq). subst.
   inverts Hvatt.
-  rewrite Hget' in Hget; inverts Hget.
-  assert (Hvp: vp = Vptr vhold_addr).
-  { clear -Hcs'.
-     unfold V_ObjPtr in *. simpl nth_val in *.
-     destruct Hcs' as [ | [ | ] ]; simpljoin; tryfalse.
-     inverts H0; auto.
-   }
-  subst.
+
+  destruct Hcs' as [Hoid | [Hhold | Hnull]].
+  
+  (***** obj_arr[idx].ptr is valid object ID *****)
+  destruct Hoid as (oid & Hoopt & Hptr & Hneq).
+  inverts Hptr.
 
   (* efield (obj_arr ′ [os_code_defs.idx ′]) ptr =ₑ p ′;ₛ *)
   rewrite Hidx_eq in *.
@@ -598,10 +584,10 @@ Proof.
 
   destruct H17 as [Hnull | ((pb & pi) & Hp)]; subst.
   destruct H16; simpljoin; tryfalse.
-  (* true If (p ′ ==ₑ NULL) *)
+
+  (* true branch for If (p ′ ==ₑ NULL) ... *)
   hoare forward.
-  pure_auto.
-  pure_auto.
+  (* exit_critical *) 
   hoare unfold.
   hoare_lifts_trms_pre (Aop, absobjs).
   eapply abscsq_rule.
@@ -646,7 +632,178 @@ Proof.
   hoare forward.
   hoare unfold.
   destruct H16; tryfalse.
-  (* false If (p ′ ==ₑ NULL)  *)
+  (* false branch for If (p ′ ==ₑ NULL) ... *)
+  hoare forward.
+  hoare unfold.
+  tryfalse.
+  instantiate (1:= Afalse).
+  hoare forward.
+  hoare unfold.
+  (* efield (obj_arr ′ [os_code_defs.idx ′]) attr =ₑ satt′ ;ₛ *)
+  hoare forward.
+  hoare_assign_array_struct.
+  (*  OSTCBCur ′ .. __OSTskLoc =ₑ ′ __Loc_normal;ₛ *)
+  unfold tcbllsegobjaux.
+  hoare_lifts_trms_pre (llsegobjaux, AOSTCBList, p_local).
+  eapply backward_rule1.
+  introv Hsat.
+  eapply tcbllsegobjaux_split3_join2_frm''; eauto.
+  hoare normal pre.
+  hoare_ex_intro.
+  hoare_split_pure_all.
+  subst.
+  hoare_assign_aux.
+  unfold isloc; auto.
+  hoare_assign_aux.
+  unfold isloc; auto.
+  unfold isptr; auto.
+  fold_aux_ptr_loc (V$ __Loc_normal) (Vnull).
+  (*  *)
+  hoare_lifts_trms_pre (Aop, absobjs).
+  eapply abscsq_rule.
+  apply noabs_oslinv.
+  eapply sobjcre_absimp_create_succ; eauto.
+  rewrite Hidx_eq; auto.
+  unfold CurTid.
+  can_change_aop_solver.
+  eapply absinfer_eq.
+  destruct H16; simpljoin; tryfalse.
+
+  eapply backward_rule1.
+  introv Hsat.
+  eapply AObjArr_select_sn_ex_strong.
+  exists v'45 (Z.to_nat idx) v'50 v'51 v'54.
+  exists (Vint32 vsatt :: Vptr (pb, pi) :: nil).
+  sep pauto; eauto.
+  rewrite <- Hlen'.
+  rewrite app_length.
+  rewrite <- list_prop1.
+  rewrite app_length.
+  simpl length. auto.
+  eapply new_array_type_vallist_match_compose_struct; auto.
+
+  lets Hcre: obj_aux_cre H19 Hloc Hptr.
+  destruct Hcre as (Hnfree & Hnref & Hkobj).
+
+  hoare forward prim.
+  unfold AOBJ.
+  unfold AObjs.
+  unfold p_local. unfold LINV, OSLInv.
+  unfold tcbllsegobjaux.
+  sep normal.
+  sep eexists.
+  sep cancel absobjs.
+  sep cancel llsegobjaux.
+  sep_lifts_trms ObjArray_P.
+  eapply astar_l_apure_intro.
+  2:{ eapply ObjArray_P_hold_for_update_to_tid_att'.
+        rewrite H27; rewrite Z2Nat.id; auto.
+        rewrite H27; rewrite Z2Nat.id; auto.
+        rewrite <- Hidx_eq; apply Int.unsigned_range_2.
+        rewrite <- Hidx_eq; apply Int.unsigned_range_2.
+        3: eauto.
+        unfolds; simpl; eauto.
+        clear -Hvp_neq. pure_auto. }
+  unfold update_nth_val.
+  sep pauto; eauto.
+  eapply objref_distinct_noref_ptr_preserve; eauto.
+  eapply objdel_nodup_set_normal_loc_preserve;
+  eapply objdel_nodup_set_null_preserve; eauto.
+  eapply objcre_nodup_set_normal_loc_preserve;
+  eapply objcre_nodup_set_null_preserve; eauto.
+  eapply obj_aux_p_cre_preserve'; eauto.
+  { introv Hf. destruct Hf as (t & Hneq_ & Htsk).
+    eapply obj_aux_del in Htsk; eauto.
+    destruct Htsk as (_ & Hf & _).
+    eapply Hf; eauto.
+  }
+  { introv Hf. destruct Hf as (t & Hneq_ & Htsk).
+    eapply objcre_nodup_cre_cre_contra; eauto.
+  }
+  eapply RH_OBJ_ECB_P_ptr_preserve; eauto.
+  unfold isloc. unfold isptr. splits; auto.
+  pure_auto.
+  hoare forward.
+  
+  (***** obj_arr[idx].ptr is a placeholder *****)
+  destruct Hhold as (Hhdeq & Hptreq).
+  subst oid_opt.
+  inverts Hptreq. 
+
+  (* efield (obj_arr ′ [os_code_defs.idx ′]) ptr =ₑ p ′;ₛ *)
+  rewrite Hidx_eq in *.
+  hoare forward.
+  hoare_assign_array_struct.
+  pure_auto.
+  rename v'52 into locmp.
+  rename v'53 into ptrmp.
+   hoare_assert_pure (get locmp tid = Some v'32 /\ get ptrmp tid = Some vr_cre).
+   { get_hsat Hsat.
+      unfold tcbllsegobjaux in Hsat.
+      sep_lifts_trms_in Hsat (llsegobjaux, AOSTCBList, p_local).
+      eapply tcbllsegobjaux_split3_join2_frm'' in Hsat; eauto.
+      sep normal in Hsat.
+      sep destruct Hsat.
+      sep split in Hsat.
+      substs.
+      split.
+      eapply join_get_r; eauto.
+      eapply join_sig_get; eauto.
+      eapply join_get_r; eauto.
+      eapply join_sig_get; eauto.
+    }
+   eapply pure_split_rule'; introv Hget_lp.
+   destruct Hget_lp as (Hloc & Hptr).
+
+  destruct H17 as [Hnull | ((pb & pi) & Hp)]; subst.
+  destruct H16; simpljoin; tryfalse.
+  (* true branch for If (p ′ ==ₑ NULL) ... *)
+  hoare forward.
+  hoare unfold.
+  hoare_lifts_trms_pre (Aop, absobjs).
+  eapply abscsq_rule.
+  apply noabs_oslinv.
+  eapply sobjcre_absimp_create_err; eauto.
+  rewrite Hidx_eq; auto.
+  can_change_aop_solver.
+  eapply absinfer_eq.
+  (*  *)
+  hoare forward prim.
+  unfold AOBJ.
+  unfold AObjs.
+  sep cancel p_local.
+  sep normal.
+  sep eexists.
+  sep cancel tcbllsegobjaux.
+  sep cancel absobjs.
+  eapply AObjArr_select_sn_ex_strong.
+  exists v'45 (Z.to_nat idx) v'50 v'51 v'54.
+  exists (Vint32 att' :: Vnull :: nil).
+  sep_lifts_trms ObjArray_P.
+  eapply astar_l_apure_intro;
+  [idtac |
+    eapply ObjArray_P_hold_for_update_to_null'; eauto;
+    try solve [rewrite <- Hidx_eq; apply Int.unsigned_range_2];
+    unfolds; simpl; eauto ].
+  unfold update_nth_val.
+  sep pauto; eauto.
+  eapply objref_distinct_objnull_preserve; eauto.
+  lets Hsame: AuxLocMod.get_set_same Hloc.
+  rewrite <- Hsame.
+  eapply obj_aux_p_objnull_preserve; eauto.
+  eapply RH_OBJ_ECB_P_null_preserve; eauto.
+  rewrite <- Hlen'.
+  rewrite app_length.
+  rewrite <- list_prop1.
+  rewrite app_length.
+  simpl length. auto.
+  eapply new_array_type_vallist_match_compose_struct; auto.
+  pure_auto.
+  hoare forward.
+  hoare forward.
+  hoare unfold.
+  destruct H16; tryfalse.
+  (* false branch for If (p ′ ==ₑ NULL)  ... *)
   hoare forward.
   pure_auto.
   pure_auto.
@@ -729,15 +886,183 @@ Proof.
   eapply objcre_nodup_set_null_preserve; eauto.
   eapply obj_aux_p_cre_preserve'; eauto.
   { introv Hf. destruct Hf as (t & Hneq & Htsk).
-     eapply obj_aux_del in Htsk; eauto.
-     destruct Htsk as (_ & Hf & _).
-     eapply Hf; eauto.
-   }
-   { introv Hf. destruct Hf as (t & Hneq & Htsk).
-      eapply objcre_nodup_cre_cre_contra; eauto.
-    }
+    eapply obj_aux_del in Htsk; eauto.
+    destruct Htsk as (_ & Hf & _).
+    eapply Hf; eauto.
+  }
+  { introv Hf. destruct Hf as (t & Hneq & Htsk).
+    eapply objcre_nodup_cre_cre_contra; eauto.
+  }
   eapply RH_OBJ_ECB_P_ptr_preserve; eauto.
   unfold isloc. unfold isptr. splits; auto.
   pure_auto.
   hoare forward.
-Qed.
+  
+  
+  (***** obj_arr[idx].ptr is null *****)
+  destruct Hnull as (Hnueq & Hptreq).
+  subst oid_opt.
+  inverts Hptreq. 
+
+  (* efield (obj_arr ′ [os_code_defs.idx ′]) ptr =ₑ p ′;ₛ *)
+  rewrite Hidx_eq in *.
+  hoare forward.
+  hoare_assign_array_struct.
+  pure_auto.
+  rename v'52 into locmp.
+  rename v'53 into ptrmp.
+   hoare_assert_pure (get locmp tid = Some v'32 /\ get ptrmp tid = Some vr_cre).
+   { get_hsat Hsat.
+      unfold tcbllsegobjaux in Hsat.
+      sep_lifts_trms_in Hsat (llsegobjaux, AOSTCBList, p_local).
+      eapply tcbllsegobjaux_split3_join2_frm'' in Hsat; eauto.
+      sep normal in Hsat.
+      sep destruct Hsat.
+      sep split in Hsat.
+      substs.
+      split.
+      eapply join_get_r; eauto.
+      eapply join_sig_get; eauto.
+      eapply join_get_r; eauto.
+      eapply join_sig_get; eauto.
+    }
+   eapply pure_split_rule'; introv Hget_lp.
+   destruct Hget_lp as (Hloc & Hptr).
+
+  destruct H17 as [Hnull | ((pb & pi) & Hp)]; subst.
+  destruct H16; simpljoin; tryfalse.
+  (* true branch for If (p ′ ==ₑ NULL) ... *)
+  hoare forward.
+  hoare unfold.
+  hoare_lifts_trms_pre (Aop, absobjs).
+  eapply abscsq_rule.
+  apply noabs_oslinv.
+  eapply sobjcre_absimp_create_err; eauto.
+  rewrite Hidx_eq; auto.
+  can_change_aop_solver.
+  eapply absinfer_eq.
+  (*  *)
+  hoare forward prim.
+  unfold AOBJ.
+  unfold AObjs.
+  sep cancel p_local.
+  sep normal.
+  sep eexists.
+  sep cancel tcbllsegobjaux.
+  sep cancel absobjs.
+  eapply AObjArr_select_sn_ex_strong.
+  exists v'45 (Z.to_nat idx) v'50 v'51 v'54.
+  exists (Vint32 att' :: Vnull :: nil).
+  sep_lifts_trms ObjArray_P.
+  eapply astar_l_apure_intro;
+  [idtac |
+    eapply ObjArray_P_hold_for_update_to_null'; eauto;
+    try solve [rewrite <- Hidx_eq; apply Int.unsigned_range_2];
+    unfolds; simpl; eauto ].
+  unfold update_nth_val.
+  sep pauto; eauto.
+  eapply objref_distinct_objnull_preserve; eauto.
+  lets Hsame: AuxLocMod.get_set_same Hloc.
+  rewrite <- Hsame.
+  eapply obj_aux_p_objnull_preserve; eauto.
+  eapply RH_OBJ_ECB_P_null_preserve; eauto.
+  go.
+  hoare forward.
+  hoare forward. 
+  hoare unfold. 
+  destruct H16; tryfalse.
+  
+  (* false branch for If (p ′ ==ₑ NULL)  ... *)
+  hoare forward.
+  hoare unfold.
+  tryfalse.
+  instantiate (1:= Afalse).
+  hoare forward.
+  hoare unfold.
+  (* efield (obj_arr ′ [os_code_defs.idx ′]) attr =ₑ satt′ ;ₛ *)
+  hoare forward.
+  hoare_assign_array_struct.
+  (*  OSTCBCur ′ .. __OSTskLoc =ₑ ′ __Loc_normal;ₛ *)
+  unfold tcbllsegobjaux.
+  hoare_lifts_trms_pre (llsegobjaux, AOSTCBList, p_local).
+  eapply backward_rule1.
+  introv Hsat.
+  eapply tcbllsegobjaux_split3_join2_frm''; eauto.
+  hoare normal pre.
+  hoare_ex_intro.
+  hoare_split_pure_all.
+  subst.
+  hoare_assign_aux.
+  unfold isloc; auto.
+  hoare_assign_aux.
+  unfold isloc; auto.
+  unfold isptr; auto.
+  fold_aux_ptr_loc (V$ __Loc_normal) (Vnull).
+  (*  *)
+  hoare_lifts_trms_pre (Aop, absobjs).
+  eapply abscsq_rule.
+  apply noabs_oslinv.
+  eapply sobjcre_absimp_create_succ; eauto.
+  rewrite Hidx_eq; auto.
+  unfold CurTid.
+  can_change_aop_solver.
+  eapply absinfer_eq.
+  destruct H16; simpljoin; tryfalse.
+
+  eapply backward_rule1.
+  introv Hsat.
+  eapply AObjArr_select_sn_ex_strong.
+  exists v'45 (Z.to_nat idx) v'50 v'51 v'54.
+  exists (Vint32 vsatt :: Vptr (pb, pi) :: nil).
+  sep pauto; eauto.
+  rewrite <- Hlen'.
+  rewrite app_length.
+  rewrite <- list_prop1.
+  rewrite app_length.
+  simpl length. auto.
+  eapply new_array_type_vallist_match_compose_struct; auto.
+
+  lets Hcre: obj_aux_cre H19 Hloc Hptr.
+  destruct Hcre as (Hnfree & Hnref & Hkobj).
+
+  hoare forward prim.
+  unfold AOBJ.
+  unfold AObjs.
+  unfold p_local. unfold LINV, OSLInv.
+  unfold tcbllsegobjaux.
+  sep normal.
+  sep eexists.
+  sep cancel absobjs.
+  sep cancel llsegobjaux.
+  sep_lifts_trms ObjArray_P.
+  eapply astar_l_apure_intro.
+  2:{ eapply ObjArray_P_hold_for_update_to_tid_att'.
+      rewrite H27; rewrite Z2Nat.id; auto.
+      rewrite H27; rewrite Z2Nat.id; auto.
+      rewrite <- Hidx_eq; apply Int.unsigned_range_2.
+      rewrite <- Hidx_eq; apply Int.unsigned_range_2.
+      3: eauto.
+      unfolds; simpl; eauto.
+      clear -Hvp_neq. pure_auto. }
+  unfold update_nth_val.
+  sep pauto; eauto.
+  eapply objref_distinct_noref_ptr_preserve; eauto.
+  eapply objdel_nodup_set_normal_loc_preserve;
+  eapply objdel_nodup_set_null_preserve; eauto.
+  eapply objcre_nodup_set_normal_loc_preserve;
+  eapply objcre_nodup_set_null_preserve; eauto.
+  eapply obj_aux_p_cre_preserve'; eauto.
+  { introv Hf. destruct Hf as (t & Hneq & Htsk).
+    eapply obj_aux_del in Htsk; eauto.
+    destruct Htsk as (_ & Hf & _).
+    eapply Hf; eauto.
+  }
+  { introv Hf. destruct Hf as (t & Hneq & Htsk).
+    eapply objcre_nodup_cre_cre_contra; eauto.
+  }
+  eapply RH_OBJ_ECB_P_ptr_preserve; eauto.
+  unfold isloc. unfold isptr. splits; auto.
+  pure_auto.
+  hoare forward.
+
+Qed.   
