certiucos/spec/obj/service_obj_oper_spec.v
@@ -61,6 +61,7 @@ Definition sobjoper_kobj_ret
      O_opt = Some O1
   end.
 
+(* the abstract program for the function **service_obj_oper** *)
 Definition sobjoper (vl: vallist) :=
   match vl with
     vidx :: vptr :: verr :: nil => 
